grind

src/Pipit.Exp.Binding.Properties.fst
@@ -19,25 +19,26 @@ module CP = Pipit.Context.Properties
 #push-options "--fuel 1 --ifuel 1"
 
 private
-let lemma_lift_lift_commute_XApp (e1: exp 'c ('b -> 'a)) (e2: exp 'c 'b) (i1: C.index { i1 <= List.Tot.length 'c }) (i2: C.index { i2 <= i1 }) (t1 t2: Type):
+let lemma_lift_lift_commute_XApp (#c: context 't) (e1: exp 't c ('b -> 'a)) (e2: exp 't c 'b) (i1: C.index_insert c) (i2: C.index { i2 <= i1 }) (t1 t2: ('t).ty):
   Lemma
     (requires (lift1' (lift1' e1 i1 t1) i2 t2 === lift1' (lift1' e1 i2 t2) (i1 + 1) t1) /\
               (lift1' (lift1' e2 i1 t1) i2 t2 === lift1' (lift1' e2 i2 t2) (i1 + 1) t1))
     (ensures (lift1' (lift1' (XApp e1 e2) i1 t1) i2 t2 === lift1' (lift1' (XApp e1 e2) i2 t2) (i1 + 1) t1))
      =
-  C.lemma_lift_lift_commute 'c i1 i2 t1 t2;
+  CP.lemma_lift_lift_commute c i1 i2 t1 t2;
   assert_norm (lift1' (lift1' (XApp e1 e2) i1 t1) i2 t2 == XApp (lift1' (lift1' e1 i1 t1) i2 t2) (lift1' (lift1' e2 i1 t1) i2 t2) );
   assert_norm ((lift1' (lift1' (XApp e1 e2) i2 t2) (i1 + 1) t1) == XApp (lift1' (lift1' e1 i2 t2) (i1 + 1) t1) (lift1' (lift1' e2 i2 t2) (i1 + 1) t1));
   ()
 
-let rec lemma_lift_lift_commute (e: exp 'c 'a) (i1: C.index { i1 <= List.Tot.length 'c }) (i2: C.index { i2 <= i1 }) (t1 t2: Type):
+let rec lemma_lift_lift_commute (#c: context 't) (e: exp 't c 'a) (i1: C.index_insert c) (i2: C.index { i2 <= i1 }) (t1 t2: ('t).ty):
   Lemma (ensures (lift1' (lift1' e i1 t1) i2 t2 === lift1' (lift1' e i2 t2) (i1 + 1) t1))
     (decreases e) =
-  C.lemma_lift_lift_commute 'c i1 i2 t1 t2;
+  CP.lemma_lift_lift_commute c i1 i2 t1 t2;
   match e with
   | XVal _ -> ()
   | XBVar _ -> ()
   | XVar _ -> ()
+  | XPrim _ -> ()
   | XApp e1 e2 ->
     lemma_lift_lift_commute e1 i1 i2 t1 t2;
     lemma_lift_lift_commute e2 i1 i2 t1 t2;
@@ -47,7 +48,7 @@ let rec lemma_lift_lift_commute (e: exp 'c 'a) (i1: C.index { i1 <= List.Tot.len
   | XThen e1 e2 ->
     lemma_lift_lift_commute e1 i1 i2 t1 t2;
     lemma_lift_lift_commute e2 i1 i2 t1 t2
-  | XMu _ e1 ->
+  | XMu e1 ->
     lemma_lift_lift_commute e1 (i1 + 1) (i2 + 1) t1 t2
   | XLet _ e1 e2 ->
     lemma_lift_lift_commute e1 i1 i2 t1 t2;
@@ -56,7 +57,7 @@ let rec lemma_lift_lift_commute (e: exp 'c 'a) (i1: C.index { i1 <= List.Tot.len
     lemma_lift_lift_commute e1 i1 i2 t1 t2;
     lemma_lift_lift_commute e2 i1 i2 t1 t2
 
-let rec lemma_subst_lift_id (e: exp 'c 'a) (i: C.index { i <= List.Tot.length 'c }) (t: Type) (p: exp 'c t):
+let rec lemma_subst_lift_id (#c: context 't) (e: exp 't c 'a) (i: C.index_insert c) (t: ('t).ty) (p: val_exp 't c t):
   Lemma (ensures (
     subst1' (lift1' e i t) i p == e))
     (decreases e) =
@@ -64,6 +65,7 @@ let rec lemma_subst_lift_id (e: exp 'c 'a) (i: C.index { i <= List.Tot.length 'c
   | XVal _ -> ()
   | XBVar _ -> ()
   | XVar _ -> ()
+  | XPrim _ -> ()
   | XApp e1 e2 ->
     assert_norm (subst1' (lift1' (XApp e1 e2) i t) i p ==
       XApp (subst1' (lift1' e1 i t) i p) (subst1' (lift1' e2 i t) i p) );
@@ -74,8 +76,8 @@ let rec lemma_subst_lift_id (e: exp 'c 'a) (i: C.index { i <= List.Tot.length 'c
   | XThen e1 e2 ->
     lemma_subst_lift_id e1 i t p;
     lemma_subst_lift_id e2 i t p
-  | XMu _ e1 ->
-    lemma_subst_lift_id e1 (i + 1) t (lift1 p 'a)
+  | XMu e1 ->
+    lemma_subst_lift_id e1 (i + 1) t (lift1 p (XMu?.valty e))
   | XLet b e1 e2 ->
     lemma_subst_lift_id e1 i t p;
     lemma_subst_lift_id e2 (i + 1) t (lift1 p b)
@@ -84,8 +86,8 @@ let rec lemma_subst_lift_id (e: exp 'c 'a) (i: C.index { i <= List.Tot.length 'c
     lemma_subst_lift_id e2 i t p
 
 private
-let _lift_of_drop (i1: C.index { C.has_index 'c i1 }) (p: exp (C.drop1 'c i1) (C.get_index 'c i1)) (t: Type):
-  exp (C.drop1 (t :: 'c) (i1 + 1)) (C.get_index (t :: 'c) (i1 + 1)) =
+let _lift_of_drop (#c: context 't) (i1: C.index_lookup c) (p: val_exp 't (C.drop1 c i1) (C.get_index c i1)) (t: ('t).ty):
+  val_exp 't (C.drop1 (t :: c) (i1 + 1)) (C.get_index (t :: c) (i1 + 1)) =
   lift1 p t
 
 (* Lift distributes over subst:
@@ -94,8 +96,8 @@ let _lift_of_drop (i1: C.index { C.has_index 'c i1 }) (p: exp (C.drop1 'c i1) (C
    These proofs are a bit involved, so I've split them out into separate lemmas
    for different cases.
 *)
-let lemma_lift_subst_distribute_le_def (e: exp 'c 'a) (i1: C.index { C.has_index 'c i1 }) (i2: C.index { i2 <= i1 }) (t2: Type) (p: exp (C.drop1 'c i1) (C.get_index 'c i1)): prop =
-    C.lemma_lift_drop_commute_le 'c i1 i2 t2;
+let lemma_lift_subst_distribute_le_def (#c: context 't) (e: exp 't c 'a) (i1: C.index_lookup c) (i2: C.index { i2 <= i1 }) (t2: ('t).ty) (p: val_exp 't (C.drop1 c i1) (C.get_index c i1)): prop =
+    CP.lemma_lift_drop_commute_le c i1 i2 t2;
     lift1' (subst1' e i1 p) i2 t2 == subst1' (lift1' e i2 t2) (i1 + 1) (lift1' p i2 t2)
 
 (* Disabling inversion seems to help solve the actual proof part, but the
@@ -103,24 +105,25 @@ let lemma_lift_subst_distribute_le_def (e: exp 'c 'a) (i1: C.index { C.has_index
    separate lemmas with inversion disabled. *)
 #push-options "--fuel 1 --ifuel 0"
 private
-let lemma_lift_subst_distribute_le_base (e: base_exp 'c 'a) (i1: C.index { C.has_index 'c i1 }) (i2: C.index { i2 <= i1 }) (t2: Type) (p: exp (C.drop1 'c i1) (C.get_index 'c i1)):
+let lemma_lift_subst_distribute_le_base (#c: context 't) (e: base_exp 't c 'a) (i1: C.index_lookup c) (i2: C.index { i2 <= i1 }) (t2: ('t).ty) (p: val_exp 't (C.drop1 c i1) (C.get_index c i1)):
   Lemma (ensures (lemma_lift_subst_distribute_le_def e i1 i2 t2 p))
     (decreases e) =
-  C.lemma_lift_drop_commute_le 'c i1 i2 t2;
-  C.lemma_lift_get_index_gt 'c i1 i2 t2;
+  CP.lemma_lift_drop_commute_le c i1 i2 t2;
+  CP.lemma_lift_get_index_gt c i1 i2 t2;
   match e with
   | XVal _ -> ()
   | XVar _ -> ()
   | XBVar i -> ()
+  | XPrim _ -> ()
 
 private
-let lemma_lift_subst_distribute_le_XApp (e1: exp 'c ('b -> 'a)) (e2: exp 'c 'b) (i1: C.index { C.has_index 'c i1 }) (i2: C.index { i2 <= i1 }) (t2: Type) (p: exp (C.drop1 'c i1) (C.get_index 'c i1)):
+let lemma_lift_subst_distribute_le_XApp (#c: context 't) (e1: exp 't c ('b -> 'a)) (e2: exp 't c 'b) (i1: C.index_lookup c) (i2: C.index { i2 <= i1 }) (t2: ('t).ty) (p: val_exp 't (C.drop1 c i1) (C.get_index c i1)):
   Lemma
     (requires (lemma_lift_subst_distribute_le_def e1 i1 i2 t2 p /\
                lemma_lift_subst_distribute_le_def e2 i1 i2 t2 p))
     (ensures (lemma_lift_subst_distribute_le_def (XApp e1 e2) i1 i2 t2 p)) =
-  C.lemma_lift_drop_commute_le 'c i1 i2 t2;
-  C.lemma_lift_get_index_gt 'c i1 i2 t2;
+  CP.lemma_lift_drop_commute_le c i1 i2 t2;
+  CP.lemma_lift_get_index_gt c i1 i2 t2;
   assert_norm (lift1' (subst1' (XApp e1 e2) i1 p) i2 t2 ==
     XApp (lift1' (subst1' e1 i1 p) i2 t2) (lift1' (subst1' e2 i1 p) i2 t2));
   assert_norm (subst1' (lift1' (XApp e1 e2) i2 t2) (i1 + 1) (lift1' p i2 t2) ==
@@ -132,13 +135,13 @@ let lemma_lift_subst_distribute_le_XApp (e1: exp 'c ('b -> 'a)) (e2: exp 'c 'b) 
 #pop-options
 
 
-let rec lemma_lift_subst_distribute_le (e: exp 'c 'a) (i1: C.index { C.has_index 'c i1 }) (i2: C.index { i2 <= i1 }) (t2: Type) (p: exp (C.drop1 'c i1) (C.get_index 'c i1)):
+let rec lemma_lift_subst_distribute_le (#c: context 't) (e: exp 't c 'a) (i1: C.index_lookup c) (i2: C.index { i2 <= i1 }) (t2: ('t).ty) (p: val_exp 't (C.drop1 c i1) (C.get_index c i1)):
   Lemma (ensures (lemma_lift_subst_distribute_le_def e i1 i2 t2 p))
     (decreases e) =
-  C.lemma_lift_drop_commute_le 'c i1 i2 t2;
-  C.lemma_lift_get_index_gt 'c i1 i2 t2;
+  CP.lemma_lift_drop_commute_le c i1 i2 t2;
+  CP.lemma_lift_get_index_gt c i1 i2 t2;
   match e with
-  | XVal _ | XVar _ | XBVar _ ->
+  | XVal _ | XVar _ | XBVar _ | XPrim _ ->
     lemma_lift_subst_distribute_le_base e i1 i2 t2 p
   | XApp e1 e2 ->
     lemma_lift_subst_distribute_le e1 i1 i2 t2 p;
@@ -151,10 +154,11 @@ let rec lemma_lift_subst_distribute_le (e: exp 'c 'a) (i1: C.index { C.has_index
     lemma_lift_subst_distribute_le e1 i1 i2 t2 p;
     lemma_lift_subst_distribute_le e2 i1 i2 t2 p;
     ()
-  | XMu _ e1 ->
-    C.lemma_lift_drop_commute_le 'c i1 0 'a;
-    lemma_lift_lift_commute p i2 0 t2 'a;
-    let p' = _lift_of_drop i1 p 'a in
+  | XMu e1 ->
+    let a' = XMu?.valty e in
+    CP.lemma_lift_drop_commute_le c i1 0 a';
+    lemma_lift_lift_commute p i2 0 t2 a';
+    let p' = _lift_of_drop i1 p a' in
     lemma_lift_subst_distribute_le e1 (i1 + 1) (i2 + 1) t2 p';
     assert (lift1' (subst1' (XMu e1) i1 p) i2 t2 ==
         subst1' (lift1' (XMu e1) i2 t2) (i1 + 1) (lift1' p i2 t2));
@@ -164,7 +168,7 @@ let rec lemma_lift_subst_distribute_le (e: exp 'c 'a) (i1: C.index { C.has_index
     lemma_lift_lift_commute p i2 0 t2 b;
     let p' = _lift_of_drop i1 p b in
 
-    C.lemma_lift_drop_commute_le 'c i1 i2 t2;
+    CP.lemma_lift_drop_commute_le c i1 i2 t2;
 
     lemma_lift_subst_distribute_le e1 i1 i2 t2 p;
     lemma_lift_subst_distribute_le e2 (i1 + 1) (i2 + 1) t2 p';
@@ -178,41 +182,47 @@ let rec lemma_lift_subst_distribute_le (e: exp 'c 'a) (i1: C.index { C.has_index
     lemma_lift_subst_distribute_le e2 i1 i2 t2 p;
     ()
 
-let lemma_subst_subst_distribute_le_def (e: exp 'c 'a) (i1: C.index { C.has_index 'c i1 }) (i2: C.index { i1 <= i2 /\ i2 < List.Tot.length 'c - 1 }) (p1: exp (C.drop1 'c i1) (C.get_index 'c i1)) (p2: exp (C.drop1 (C.drop1 'c i1) i2) (C.get_index (C.drop1 'c i1) i2)) =
-    C.lemma_drop_drop_commute 'c i1 i2;
-    C.lemma_drop_get_index_lt 'c (i2 + 1) i1;
+let lemma_subst_subst_distribute_le_def (#c: context 't) (e: exp 't c 'a) (i1: C.index_lookup c) (i2: C.index { i1 <= i2 /\ i2 < List.Tot.length c - 1 }) (p1: val_exp 't (C.drop1 c i1) (C.get_index c i1)) (p2: val_exp 't (C.drop1 (C.drop1 c i1) i2) (C.get_index (C.drop1 c i1) i2)) =
+    CP.lemma_drop_drop_commute c i1 i2;
+    CP.lemma_drop_get_index_lt c (i2 + 1) i1;
     subst1' (subst1' e i1 p1) i2 p2 ==
-    subst1' (subst1' e (i2 + 1) (lift1' p2 i1 (C.get_index 'c i1))) i1 (subst1' p1 i2 p2)
+    subst1' (subst1' e (i2 + 1) (lift1' p2 i1 (C.get_index c i1))) i1 (subst1' p1 i2 p2)
+
+let lemma_exp_invert_XBVar (#c: context 't) (e: exp 't c 'a { XBVar? e }):
+  Lemma ('a == ('t).ty_sem (C.get_index c (XBVar?.i e))) =
+  ()
 
 #push-options "--fuel 1 --ifuel 0"
 
 private
-let lemma_subst_subst_distribute_le_base (e: base_exp 'c 'a) (i1: C.index { C.has_index 'c i1 }) (i2: C.index { i1 <= i2 /\ i2 < List.Tot.length 'c - 1 }) (p1: exp (C.drop1 'c i1) (C.get_index 'c i1)) (p2: exp (C.drop1 (C.drop1 'c i1) i2) (C.get_index (C.drop1 'c i1) i2)):
+let lemma_subst_subst_distribute_le_base (#c: context 't) (e: base_exp 't c 'a) (i1: C.index_lookup c) (i2: C.index { i1 <= i2 /\ i2 < List.Tot.length c - 1 }) (p1: val_exp 't (C.drop1 c i1) (C.get_index c i1)) (p2: val_exp 't (C.drop1 (C.drop1 c i1) i2) (C.get_index (C.drop1 c i1) i2)):
   Lemma (ensures
     lemma_subst_subst_distribute_le_def e i1 i2 p1 p2) =
-  C.lemma_drop_drop_commute 'c i1 i2;
-  C.lemma_drop_get_index_lt 'c (i2 + 1) i1;
+  CP.lemma_drop_drop_commute c i1 i2;
+  CP.lemma_drop_get_index_lt c (i2 + 1) i1;
   match e with
   | XVal v -> ()
   | XVar _ -> ()
+  | XPrim _ -> ()
   | XBVar i' ->
     if i' = i1
     then ()
     else if i' = i2 + 1
     then begin
+      lemma_exp_invert_XBVar e;
       calc (==) {
-        C.lift1 (C.drop1 (C.drop1 'c i1) i2) i1 (C.get_index 'c i1);
-        (==) { C.lemma_lift_drop_commute_le (C.drop1 'c i1) i2 i1 (C.get_index 'c i1) }
-        C.drop1 (C.lift1 (C.drop1 'c i1) i1 (C.get_index 'c i1)) (i2 + 1);
-        (==) { C.lemma_lift_drop_eq 'c i1 }
-        C.drop1 'c (i2 + 1);
+        C.lift1 (C.drop1 (C.drop1 c i1) i2) i1 (C.get_index c i1);
+        (==) { CP.lemma_lift_drop_commute_le (C.drop1 c i1) i2 i1 (C.get_index c i1) }
+        C.drop1 (C.lift1 (C.drop1 c i1) i1 (C.get_index c i1)) (i2 + 1);
+        (==) { CP.lemma_lift_drop_eq c i1 }
+        C.drop1 c (i2 + 1);
       };
-      let p2': exp (C.drop1 'c (i2 + 1)) (C.get_index (C.drop1 'c i1) i2) = coerce_eq () (lift1' p2 i1 (C.get_index 'c i1)) in
+      let p2': val_exp 't (C.drop1 c (i2 + 1)) (C.get_index (C.drop1 c i1) i2) = coerce_eq () (lift1' p2 i1 (C.get_index c i1)) in
       calc (==) {
         subst1' (subst1' e (i2 + 1) p2') i1 (subst1' p1 i2 p2);
         (==) { }
-        subst1' (lift1' p2 i1 (C.get_index 'c i1)) i1 (subst1' p1 i2 p2);
-        (==) { lemma_subst_lift_id p2 i1 (C.get_index 'c i1) (subst1' p1 i2 p2) }
+        subst1' (lift1' p2 i1 (C.get_index c i1)) i1 (subst1' p1 i2 p2);
+        (==) { lemma_subst_lift_id p2 i1 (C.get_index c i1) (subst1' p1 i2 p2) }
         p2;
       };
       ()
@@ -220,107 +230,110 @@ let lemma_subst_subst_distribute_le_base (e: base_exp 'c 'a) (i1: C.index { C.ha
     else ()
 
 private
-let lemma_subst_subst_distribute_le_XApp
-  (e1: exp 'c ('b -> 'a)) (e2: exp 'c 'b) (i1: C.index { C.has_index 'c i1 }) (i2: C.index { i1 <= i2 /\ i2 < List.Tot.length 'c - 1 }) (p1: exp (C.drop1 'c i1) (C.get_index 'c i1)) (p2: exp (C.drop1 (C.drop1 'c i1) i2) (C.get_index (C.drop1 'c i1) i2)):
+let lemma_subst_subst_distribute_le_XApp (#c: context 't)
+  (e1: exp 't c ('b -> 'a)) (e2: exp 't c 'b) (i1: C.index_lookup c) (i2: C.index { i1 <= i2 /\ i2 < List.Tot.length c - 1 }) (p1: val_exp 't (C.drop1 c i1) (C.get_index c i1)) (p2: val_exp 't (C.drop1 (C.drop1 c i1) i2) (C.get_index (C.drop1 c i1) i2)):
   Lemma
     (requires (lemma_subst_subst_distribute_le_def e1 i1 i2 p1 p2 /\
                lemma_subst_subst_distribute_le_def e2 i1 i2 p1 p2))
     (ensures (lemma_subst_subst_distribute_le_def (XApp e1 e2) i1 i2 p1 p2)) =
-  C.lemma_drop_drop_commute 'c i1 i2;
-  C.lemma_drop_get_index_lt 'c (i2 + 1) i1;
+  CP.lemma_drop_drop_commute c i1 i2;
+  CP.lemma_drop_get_index_lt c (i2 + 1) i1;
   assert_norm (subst1' (subst1' (XApp e1 e2) i1 p1) i2 p2 ==
     XApp (subst1' (subst1' e1 i1 p1) i2 p2) (subst1' (subst1' e2 i1 p1) i2 p2));
-  assert_norm (subst1' (subst1' (XApp e1 e2) (i2 + 1) (lift1' p2 i1 (C.get_index 'c i1))) i1 (subst1' p1 i2 p2) ==
-    XApp (subst1' (subst1' e1 (i2 + 1) (lift1' p2 i1 (C.get_index 'c i1))) i1 (subst1' p1 i2 p2)) (subst1' (subst1' e2 (i2 + 1) (lift1' p2 i1 (C.get_index 'c i1))) i1 (subst1' p1 i2 p2)));
+  assert_norm (subst1' (subst1' (XApp e1 e2) (i2 + 1) (lift1' p2 i1 (C.get_index c i1))) i1 (subst1' p1 i2 p2) ==
+    XApp (subst1' (subst1' e1 (i2 + 1) (lift1' p2 i1 (C.get_index c i1))) i1 (subst1' p1 i2 p2)) (subst1' (subst1' e2 (i2 + 1) (lift1' p2 i1 (C.get_index c i1))) i1 (subst1' p1 i2 p2)));
   ()
 
 private
 let lemma_subst_subst_distribute_le_XMu
-  {| Pipit.Inhabited.inhabited 'a |}
-  (e: exp ('a :: 'c) 'a) (i1: C.index { C.has_index 'c i1 }) (i2: C.index { i1 <= i2 /\ i2 < List.Tot.length 'c - 1 }) (p1: exp (C.drop1 'c i1) (C.get_index 'c i1)) (p2: exp (C.drop1 (C.drop1 'c i1) i2) (C.get_index (C.drop1 'c i1) i2)):
+  (#c: context 't)
+  (#te: ('t).ty)
+  (e: val_exp 't (te :: c) te) (i1: C.index_lookup c) (i2: C.index { i1 <= i2 /\ i2 < List.Tot.length c - 1 }) (p1: val_exp 't (C.drop1 c i1) (C.get_index c i1)) (p2: val_exp 't (C.drop1 (C.drop1 c i1) i2) (C.get_index (C.drop1 c i1) i2)):
   Lemma
-    (requires (lemma_subst_subst_distribute_le_def e (i1 + 1) (i2 + 1) (_lift_of_drop i1 p1 'a) (_lift_of_drop i2 p2 'a)))
+    (requires (lemma_subst_subst_distribute_le_def e (i1 + 1) (i2 + 1) (_lift_of_drop i1 p1 te) (_lift_of_drop i2 p2 te)))
     (ensures (lemma_subst_subst_distribute_le_def (XMu e) i1 i2 p1 p2)) =
-    let p1' = _lift_of_drop i1 p1 'a in
-    let p2' = _lift_of_drop i2 p2 'a in
-    lemma_lift_lift_commute p2 i1 0 (C.get_index 'c i1) 'a;
-    lemma_lift_subst_distribute_le p1 i2 0 'a p2;
+    let p1' = _lift_of_drop i1 p1 te in
+    let p2' = _lift_of_drop i2 p2 te in
+    lemma_lift_lift_commute p2 i1 0 (C.get_index c i1) te;
+    lemma_lift_subst_distribute_le p1 i2 0 te p2;
 
-    C.lemma_lift_drop_commute_le (C.drop1 'c i1) i2 i1 (C.get_index 'c i1);
-    C.lemma_lift_drop_eq 'c i1;
+    CP.lemma_lift_drop_commute_le (C.drop1 c i1) i2 i1 (C.get_index c i1);
+    CP.lemma_lift_drop_eq c i1;
 
-    C.lemma_dropCons 'a 'c (i2 + 2);
-    C.lemma_dropCons 'a (C.drop1 'c (i2 + 1)) (i1 + 1);
-    assert ('a :: C.drop1 (C.drop1 'c (i2 + 1)) i1 == C.drop1 (C.drop1 ('a :: 'c) (i2 + 2)) (i1 + 1));
-    assert (C.get_index ('a :: 'c) (i2 + 2) == C.get_index ('a :: C.drop1 'c i1) (i2 + 1));
-    C.lemma_dropCons 'a 'c (i2 + 1);
-    C.lemma_dropCons 'a (C.drop1 'c i1) (i2 + 1);
-    assert (C.drop1 ('a :: 'c) (i2 + 2) == C.lift1 (C.drop1 ('a :: C.drop1 'c i1) (i2 + 1)) (i1 + 1) (C.get_index 'c i1));
+    CP.lemma_dropCons te c (i2 + 2);
+    CP.lemma_dropCons te (C.drop1 c (i2 + 1)) (i1 + 1);
+    assert (te :: C.drop1 (C.drop1 c (i2 + 1)) i1 == C.drop1 (C.drop1 (te :: c) (i2 + 2)) (i1 + 1));
+    assert (C.get_index (te :: c) (i2 + 2) == C.get_index (te :: C.drop1 c i1) (i2 + 1));
+    CP.lemma_dropCons te c (i2 + 1);
+    CP.lemma_dropCons te (C.drop1 c i1) (i2 + 1);
+    assert (C.drop1 (te :: c) (i2 + 2) == C.lift1 (C.drop1 (te :: C.drop1 c i1) (i2 + 1)) (i1 + 1) (C.get_index c i1));
 
-    C.lemma_drop_drop_commute 'c i1 i2;
-    C.lemma_drop_get_index_lt 'c (i2 + 1) i1;
+    CP.lemma_drop_drop_commute c i1 i2;
+    CP.lemma_drop_get_index_lt c (i2 + 1) i1;
     assert (subst1' (subst1' (XMu e) i1 p1) i2 p2 ==
             XMu (subst1' (subst1' e (i1 + 1) p1') (i2 + 1) p2'));
     assert (XMu (coerce_eq () (subst1' (subst1' e (i1 + 1) p1') (i2 + 1) p2')) ==
-            XMu #(C.drop1 (C.drop1 'c (i2 + 1)) i1) (subst1' (subst1' e (i2 + 2) (lift1' p2' (i1 + 1) (C.get_index 'c i1))) (i1 + 1) (subst1' p1' (i2 + 1) p2')));
-    assert (subst1' (subst1' (XMu e) (i2 + 1) (lift1' p2 i1 (C.get_index 'c i1))) i1 (subst1' p1 i2 p2) ==
-            XMu (subst1' (subst1' e (i2 + 2) (lift1 (lift1' p2 i1 (C.get_index 'c i1)) 'a)) (i1 + 1) (lift1 (subst1' p1 i2 p2) 'a)));
+            XMu #'t #(C.drop1 (C.drop1 c (i2 + 1)) i1) (subst1' (subst1' e (i2 + 2) (lift1' p2' (i1 + 1) (C.get_index c i1))) (i1 + 1) (subst1' p1' (i2 + 1) p2')));
+    assert (subst1' (subst1' (XMu e) (i2 + 1) (lift1' p2 i1 (C.get_index c i1))) i1 (subst1' p1 i2 p2) ==
+            XMu (subst1' (subst1' e (i2 + 2) (lift1 (lift1' p2 i1 (C.get_index c i1)) te)) (i1 + 1) (lift1 (subst1' p1 i2 p2) te)));
     assert (subst1' (subst1' (XMu e) i1 p1) i2 p2 ==
-            subst1' (subst1' (XMu e) (i2 + 1) (lift1' p2 i1 (C.get_index 'c i1))) i1 (subst1' p1 i2 p2));
+            subst1' (subst1' (XMu e) (i2 + 1) (lift1' p2 i1 (C.get_index c i1))) i1 (subst1' p1 i2 p2));
 
     ()
 
 private
 let lemma_subst_subst_distribute_le_XLet
-  (e1: exp 'c 'b) (e2: exp ('b :: 'c) 'a) (i1: C.index { C.has_index 'c i1 }) (i2: C.index { i1 <= i2 /\ i2 < List.Tot.length 'c - 1 }) (p1: exp (C.drop1 'c i1) (C.get_index 'c i1)) (p2: exp (C.drop1 (C.drop1 'c i1) i2) (C.get_index (C.drop1 'c i1) i2)):
+  (#c: context 't)
+  (#t1: ('t).ty)
+  (e1: val_exp 't c t1) (e2: exp 't (t1 :: c) 'a) (i1: C.index_lookup c) (i2: C.index { i1 <= i2 /\ i2 < List.Tot.length c - 1 }) (p1: val_exp 't (C.drop1 c i1) (C.get_index c i1)) (p2: val_exp 't (C.drop1 (C.drop1 c i1) i2) (C.get_index (C.drop1 c i1) i2)):
   Lemma
     (requires (lemma_subst_subst_distribute_le_def e1 i1 i2 p1 p2 /\
-               lemma_subst_subst_distribute_le_def e2 (i1 + 1) (i2 + 1) (_lift_of_drop i1 p1 'b) (coerce_eq () (_lift_of_drop i2 p2 'b))))
-    (ensures (lemma_subst_subst_distribute_le_def (XLet 'b e1 e2) i1 i2 p1 p2)) =
-    let p1' = _lift_of_drop i1 p1 'b in
-    let p2' = _lift_of_drop i2 p2 'b in
-    lemma_lift_lift_commute p2 i1 0 (C.get_index 'c i1) 'b;
-    lemma_lift_subst_distribute_le p1 i2 0 'b p2;
+               lemma_subst_subst_distribute_le_def e2 (i1 + 1) (i2 + 1) (_lift_of_drop i1 p1 t1) (coerce_eq () (_lift_of_drop i2 p2 t1))))
+    (ensures (lemma_subst_subst_distribute_le_def (XLet #'t t1 e1 e2) i1 i2 p1 p2)) =
+    let p1' = _lift_of_drop i1 p1 t1 in
+    let p2' = _lift_of_drop i2 p2 t1 in
+    lemma_lift_lift_commute p2 i1 0 (C.get_index c i1) t1;
+    lemma_lift_subst_distribute_le p1 i2 0 t1 p2;
 
-    C.lemma_lift_drop_commute_le (C.drop1 'c i1) i2 i1 (C.get_index 'c i1);
-    C.lemma_lift_drop_eq 'c i1;
+    CP.lemma_lift_drop_commute_le (C.drop1 c i1) i2 i1 (C.get_index c i1);
+    CP.lemma_lift_drop_eq c i1;
 
-    C.lemma_dropCons 'b 'c (i2 + 2);
-    C.lemma_dropCons 'b (C.drop1 'c (i2 + 1)) (i1 + 1);
-    assert ('b :: C.drop1 (C.drop1 'c (i2 + 1)) i1 == C.drop1 (C.drop1 ('b :: 'c) (i2 + 2)) (i1 + 1));
-    assert (C.get_index ('b :: 'c) (i2 + 2) == C.get_index ('b :: C.drop1 'c i1) (i2 + 1));
-    C.lemma_dropCons 'b 'c (i2 + 1);
-    C.lemma_dropCons 'b (C.drop1 'c i1) (i2 + 1);
-    assert (C.drop1 ('b :: 'c) (i2 + 2) == C.lift1 (C.drop1 ('b :: C.drop1 'c i1) (i2 + 1)) (i1 + 1) (C.get_index 'c i1));
+    CP.lemma_dropCons t1 c (i2 + 2);
+    CP.lemma_dropCons t1 (C.drop1 c (i2 + 1)) (i1 + 1);
+    assert (t1 :: C.drop1 (C.drop1 c (i2 + 1)) i1 == C.drop1 (C.drop1 (t1 :: c) (i2 + 2)) (i1 + 1));
+    assert (C.get_index (t1 :: c) (i2 + 2) == C.get_index (t1 :: C.drop1 c i1) (i2 + 1));
+    CP.lemma_dropCons t1 c (i2 + 1);
+    CP.lemma_dropCons t1 (C.drop1 c i1) (i2 + 1);
+    assert (C.drop1 (t1 :: c) (i2 + 2) == C.lift1 (C.drop1 (t1 :: C.drop1 c i1) (i2 + 1)) (i1 + 1) (C.get_index c i1));
 
-    C.lemma_drop_drop_commute 'c i1 i2;
-    C.lemma_drop_get_index_lt 'c (i2 + 1) i1;
+    CP.lemma_drop_drop_commute c i1 i2;
+    CP.lemma_drop_get_index_lt c (i2 + 1) i1;
 
     let e1'l = subst1' (subst1' e1 i1 p1) i2 p2 in
     let e2'l = subst1' (subst1' e2 (i1 + 1) p1') (i2 + 1) p2' in
 
-    assert (subst1' (subst1' (XLet 'b e1 e2) i1 p1) i2 p2 ==
-            XLet 'b e1'l e2'l);
-    assert (XLet 'b e1'l e2'l ==
-            XLet #(C.drop1 (C.drop1 'c (i2 + 1)) i1) 'b e1'l (subst1' (subst1' e2 (i2 + 2) (lift1' p2' (i1 + 1) (C.get_index 'c i1))) (i1 + 1) (subst1' p1' (i2 + 1) p2')));
-    assert (subst1' (subst1' (XLet 'b e1 e2) (i2 + 1) (lift1' p2 i1 (C.get_index 'c i1))) i1 (subst1' p1 i2 p2) ==
-            XLet 'b (subst1' (subst1' e1 (i2 + 1) (lift1' p2 i1 (C.get_index 'c i1))) i1 (subst1' p1 i2 p2)) (subst1' (subst1' e2 (i2 + 2) (lift1 (lift1' p2 i1 (C.get_index 'c i1)) 'b)) (i1 + 1) (lift1 (subst1' p1 i2 p2) 'b)));
-    assert (subst1' (subst1' (XLet 'b e1 e2) i1 p1) i2 p2 ==
-            subst1' (subst1' (XLet 'b e1 e2) (i2 + 1) (lift1' p2 i1 (C.get_index 'c i1))) i1 (subst1' p1 i2 p2));
+    assert (subst1' (subst1' (XLet t1 e1 e2) i1 p1) i2 p2 ==
+            XLet t1 e1'l e2'l);
+    assert (XLet t1 e1'l e2'l ==
+            XLet #'t #(C.drop1 (C.drop1 c (i2 + 1)) i1) t1 e1'l (subst1' (subst1' e2 (i2 + 2) (lift1' p2' (i1 + 1) (C.get_index c i1))) (i1 + 1) (subst1' p1' (i2 + 1) p2')));
+    assert (subst1' (subst1' (XLet t1 e1 e2) (i2 + 1) (lift1' p2 i1 (C.get_index c i1))) i1 (subst1' p1 i2 p2) ==
+            XLet t1 (subst1' (subst1' e1 (i2 + 1) (lift1' p2 i1 (C.get_index c i1))) i1 (subst1' p1 i2 p2)) (subst1' (subst1' e2 (i2 + 2) (lift1 (lift1' p2 i1 (C.get_index c i1)) t1)) (i1 + 1) (lift1 (subst1' p1 i2 p2) t1)));
+    assert (subst1' (subst1' (XLet t1 e1 e2) i1 p1) i2 p2 ==
+            subst1' (subst1' (XLet t1 e1 e2) (i2 + 1) (lift1' p2 i1 (C.get_index c i1))) i1 (subst1' p1 i2 p2));
 
     ()
 
 #push-options "--fuel 1 --ifuel 1"
 
-let rec lemma_subst_subst_distribute_le (e: exp 'c 'a) (i1: C.index { C.has_index 'c i1 }) (i2: C.index { i1 <= i2 /\ i2 < List.Tot.length 'c - 1 }) (p1: exp (C.drop1 'c i1) (C.get_index 'c i1)) (p2: exp (C.drop1 (C.drop1 'c i1) i2) (C.get_index (C.drop1 'c i1) i2)):
+let rec lemma_subst_subst_distribute_le (#c: context 't) (e: exp 't c 'a) (i1: C.index_lookup c) (i2: C.index { i1 <= i2 /\ i2 < List.Tot.length c - 1 }) (p1: val_exp 't (C.drop1 c i1) (C.get_index c i1)) (p2: val_exp 't (C.drop1 (C.drop1 c i1) i2) (C.get_index (C.drop1 c i1) i2)):
   Lemma (ensures
-    (C.lemma_drop_drop_commute 'c i1 i2;
-    C.lemma_drop_get_index_lt 'c (i2 + 1) i1;
+    (CP.lemma_drop_drop_commute c i1 i2;
+    CP.lemma_drop_get_index_lt c (i2 + 1) i1;
     subst1' (subst1' e i1 p1) i2 p2 ==
-    subst1' (subst1' e (i2 + 1) (lift1' p2 i1 (C.get_index 'c i1))) i1 (subst1' p1 i2 p2)))
+    subst1' (subst1' e (i2 + 1) (lift1' p2 i1 (C.get_index c i1))) i1 (subst1' p1 i2 p2)))
     (decreases e) =
-  C.lemma_drop_drop_commute 'c i1 i2;
-  C.lemma_drop_get_index_lt 'c (i2 + 1) i1;
+  CP.lemma_drop_drop_commute c i1 i2;
+  CP.lemma_drop_get_index_lt c (i2 + 1) i1;
   match e with
   | XVal _ | XVar _ | XBVar _ -> lemma_subst_subst_distribute_le_base e i1 i2 p1 p2
 
@@ -340,9 +353,10 @@ let rec lemma_subst_subst_distribute_le (e: exp 'c 'a) (i1: C.index { C.has_inde
     lemma_subst_subst_distribute_le e2 i1 i2 p1 p2;
     ()
 
-  | XMu _ e1 ->
-    let p1' = _lift_of_drop i1 p1 'a in
-    let p2' = _lift_of_drop i2 p2 'a in
+  | XMu e1 ->
+    let valty = XMu?.valty e in
+    let p1' = _lift_of_drop i1 p1 valty in
+    let p2' = _lift_of_drop i2 p2 valty in
     lemma_subst_subst_distribute_le e1 (i1 + 1) (i2 + 1) p1' p2';
     lemma_subst_subst_distribute_le_XMu e1 i1 i2 p1 p2
   | XLet b e1 e2 ->
@@ -352,9 +366,9 @@ let rec lemma_subst_subst_distribute_le (e: exp 'c 'a) (i1: C.index { C.has_inde
     lemma_subst_subst_distribute_le e2 (i1 + 1) (i2 + 1) p1' p2';
     lemma_subst_subst_distribute_le_XLet e1 e2 i1 i2 p1 p2
 
-let lemma_subst_subst_distribute_XMu {| Pipit.Inhabited.inhabited 'a |} (e: exp ('a :: 'c) 'a) (i: C.index { C.has_index 'c i }) (p: exp (C.drop1 'c i) (C.get_index 'c i)):
+let lemma_subst_subst_distribute_XMu (#c: context 't) (#te: ('t).ty) (e: val_exp 't (te :: c) te) (i: C.index_lookup c) (p: val_exp 't (C.drop1 c i) (C.get_index c i)):
   Lemma (ensures
     subst1' (subst1 e (XMu e)) i p ==
-    subst1 (subst1' e (i + 1) (lift1 p 'a)) (XMu (subst1' e (i + 1) (lift1 p 'a))))
+    subst1 (subst1' e (i + 1) (lift1 p te)) (XMu (subst1' e (i + 1) (lift1 p te))))
     =
   lemma_subst_subst_distribute_le e 0 i (XMu e) p
